rocq-brick-libstdcpp/proof/ctime/pred.v
@@ -8,42 +8,47 @@ Require Import skylabs.auto.cpp.elpi.derive.
 Require Export skylabs.cpp.string.
 Require Export skylabs.brick.libstdcpp.iostream.pred.
 
+Require Export skylabs.brick.libstdcpp.ctime.model.
 Require Import skylabs.brick.libstdcpp.ctime.inc_ctime_cpp.
 
 #[local] Set Primitive Projections.
 
-Record tm_model := {
-  tm_model_sec : Z;
-  tm_model_min : Z;
-  tm_model_hour : Z;
-  tm_model_mday : Z;
-  tm_model_mon : Z;
-  tm_model_year : Z;
-  tm_model_wday : Z;
-  tm_model_yday : Z;
-  tm_model_isdst : Z;
-}.
-
-Record timespec_model := {
-  timespec_model_sec : Z;
-  timespec_model_nsec : Z;
-}.
-
 Section with_cpp.
   Context `{Σ : cpp_logic, σ : genv}.
 
+  Parameter later_than : abs_time -> mpred.
+  Parameter later_than_knowledge : Knowledge1 later_than.
+  Parameter later_than_timeless : Timeless1 later_than.
+  Parameter later_than_weakly_objective : WeaklyObjective1 later_than.
+  Axiom later_than_down_closed :
+    forall t1 t2,
+      (t1 <= t2)%N ->
+      later_than (abs_time_of_N t2) |-- later_than (abs_time_of_N t1).
+
+  #[global] Existing Instance later_than_knowledge.
+  #[global] Existing Instance later_than_timeless.
+  #[global] Existing Instance later_than_weakly_objective.
+
+  (* TODO: Investigate whether [tm_zone] should be owned, borrowed, or abstracted away. *)
   Parameter tmR_hidden :
-    cQp.t -> tm_model -> Z -> cstring.t -> Rep.
+    cQp.t -> tm_model -> Rep.
   #[only(type_ptr="tm", cfracsplittable)] derive tmR_hidden.
 
-  Definition tmR (q : cQp.t) (tm : tm_model) : Rep :=
-    Exists gmtoff zone,
-      tmR_hidden q tm gmtoff zone.
-
-  Parameter timespecR : cQp.t -> timespec_model -> Rep.
-  #[only(type_ptr="timespec", cfracsplittable)] derive timespecR.
-
-  #[global] Instance timespecR_learnable : LearnEqF1 timespecR :=
-    ltac:(solve_learnable).
-
+  Parameter timespecR_raw : cQp.t -> timespec_model -> Rep.
+  #[only(type_ptr="timespec", cfracsplittable)] derive timespecR_raw.
 End with_cpp.
+
+sl.lock
+Definition tmR `{Σ : cpp_logic} {σ : genv} (q : cQp.t) (tm : tm_model) : Rep :=
+  tmR_hidden q tm.
+#[only(lazy_unfold)] derive tmR.
+#[only(type_ptr,cfracsplittable)] derive tmR.
+
+sl.lock
+Definition timespecR `{Σ : cpp_logic} {σ : genv} (q : cQp.t) (ts : timespec_model) : Rep :=
+  timespecR_raw q ts.
+#[only(lazy_unfold)] derive timespecR.
+#[only(type_ptr,cfracsplittable)] derive timespecR.
+
+#[global] Instance timespecR_learnable `{Σ : cpp_logic} {σ : genv} : LearnEqF1 timespecR :=
+  ltac:(solve_learnable).
